theories/Theorems/Order.v
@@ -3,6 +3,7 @@ From Coq Require Import Lists.List. Import ListNotations.
 From Coq Require Import NArith.BinNat.
 From Coq Require Import Hexadecimal.
 From Coq Require Import Strings.Byte.
+From Coq Require Import Arith.
 From Coq Require Import Lia.
 
 Ltac crush_bits :=
@@ -50,35 +51,88 @@ Definition nth_valid_codepoint (n: N) : option codepoint :=
   else
     None.
 
-Lemma nth_valid_codepoint_is_some_implies_valid : forall n code,
-    nth_valid_codepoint n = Some code ->
-    valid_codepoint code.
+Lemma nth_valid_codepoint_is_some_implies_valid : forall code,
+    (exists n, nth_valid_codepoint n = Some code) <->
+      valid_codepoint code.
 Proof.
-  intros n code nth.
-  unfold valid_codepoint, codepoint_less_than_10ffff, codepoint_is_not_surrogate.
-  unfold nth_valid_codepoint in nth.
-  destruct (n <? cd800)%N eqn:less_than_d800; inversion nth; subst; clear nth.
-  - apply N.ltb_lt in less_than_d800.
-    split. apply N.lt_le_incl in less_than_d800. apply N.le_trans with (m:= cd800). assumption. vm_compute. easy.
-    left. assumption.
-  - apply N.ltb_nlt in less_than_d800.
-    destruct (n <=? 1112063)%N eqn:less_than_10ffff_m_800; [| discriminate].
-    apply N.leb_le in less_than_10ffff_m_800.
-    inversion H0. subst. clear H0.
-    split. replace (1112063)%N with (c10ffff - c0800)%N in less_than_10ffff_m_800 by reflexivity.
-    specialize (N.add_le_mono_r n (c10ffff - c0800)%N c0800) as [G1 G2].
-    apply G1 in less_than_10ffff_m_800.
-    rewrite N.sub_add in less_than_10ffff_m_800.
-    apply less_than_10ffff_m_800. vm_compute. intro. discriminate.
-    apply N.nlt_ge in less_than_d800.
-    right. apply N.lt_gt.
-    specialize (N.add_le_mono_r cd800 n c0800) as [G1 G2].
-    apply G1 in less_than_d800.
-    replace (cd800 + c0800)%N with (ce000) in less_than_d800 by reflexivity.
-    specialize (N.lt_succ_diag_r cdfff) as s. replace (N.succ cdfff) with ce000 in s by reflexivity.
-    lia.
+  intros code. split. 
+  - intro nth. destruct nth as [n nth].
+    unfold valid_codepoint, codepoint_less_than_10ffff, codepoint_is_not_surrogate.
+    unfold nth_valid_codepoint in nth.
+    destruct (n <? cd800)%N eqn:less_than_d800; inversion nth; subst; clear nth.
+    + apply N.ltb_lt in less_than_d800.
+      split. apply N.lt_le_incl in less_than_d800. apply N.le_trans with (m:= cd800). assumption. vm_compute. easy.
+      left. assumption.
+    + apply N.ltb_nlt in less_than_d800.
+      destruct (n <=? 1112063)%N eqn:less_than_10ffff_m_800; [| discriminate].
+      apply N.leb_le in less_than_10ffff_m_800.
+      inversion H0. subst. clear H0.
+      split. replace (1112063)%N with (c10ffff - c0800)%N in less_than_10ffff_m_800 by reflexivity.
+      specialize (N.add_le_mono_r n (c10ffff - c0800)%N c0800) as [G1 G2].
+      apply G1 in less_than_10ffff_m_800.
+      rewrite N.sub_add in less_than_10ffff_m_800.
+      apply less_than_10ffff_m_800. vm_compute. intro. discriminate.
+      apply N.nlt_ge in less_than_d800.
+      right. apply N.lt_gt.
+      specialize (N.add_le_mono_r cd800 n c0800) as [G1 G2].
+      apply G1 in less_than_d800.
+      replace (cd800 + c0800)%N with (ce000) in less_than_d800 by reflexivity.
+      specialize (N.lt_succ_diag_r cdfff) as s. replace (N.succ cdfff) with ce000 in s by reflexivity.
+      lia.
+  - intro valid_code.
+    unfold valid_codepoint, codepoint_less_than_10ffff, codepoint_is_not_surrogate in valid_code.
+    destruct valid_code as [code_less_10ffff code_not_surrogate].
+    unfold nth_valid_codepoint.
+    destruct code_not_surrogate.
+    + exists code. apply <- N.ltb_lt in H. rewrite H. reflexivity.
+    + exists (code - c0800)%N.
+      destruct (code - c0800 <? cd800)%N eqn:less_d800.
+      * apply N.ltb_lt in less_d800. specialize (N.add_lt_mono_r (code - c0800)%N cd800 c0800) as [G1 G2].
+        apply G1 in less_d800. rewrite N.sub_add in less_d800.
+        replace (cd800 + c0800)%N with (N.succ cdfff) in less_d800 by reflexivity. lia.
+        apply N.gt_lt in H. apply N.lt_le_incl in H. apply N.le_trans with (m := cdfff). vm_compute. intro. discriminate.
+        assumption.
+      * apply N.ltb_nlt in less_d800.
+        destruct (code - c0800 <=? c10ffff - c0800)%N eqn: less_c10ffff_m_800.
+        -- rewrite N.sub_add. reflexivity.
+           apply N.gt_lt in H. apply N.lt_le_incl in H. apply N.le_trans with (m := cdfff). vm_compute. intro. discriminate. assumption.
+        -- apply N.leb_nle in less_c10ffff_m_800.
+           apply N.lt_nge in less_c10ffff_m_800.
+           apply N.lt_sub_lt_add_r in less_c10ffff_m_800. rewrite N.sub_add in less_c10ffff_m_800.
+           lia. apply N.gt_lt in H. apply N.lt_le_incl in H. apply N.le_trans with (m := cdfff). vm_compute. intro. discriminate. assumption.
 Qed.
-    
+
+Theorem nth_valid_codepoint_compat : forall n1 code1 n2 code2,
+    nth_valid_codepoint n1 = Some code1 ->
+    nth_valid_codepoint n2 = Some code2 ->
+    N.compare n1 n2 = N.compare code1 code2.
+Proof.
+  intros n1 code1 n2 code2 code1_valid code2_valid.
+  unfold nth_valid_codepoint in code1_valid, code2_valid.
+  repeat match goal with
+  | [G: context[if (?a <=? ?b)%N then _ else _] |- _] => 
+      let l := fresh "less_than_eq" in
+      destruct (a <=? b)%N eqn:l; [apply N.leb_le in l| apply N.leb_nle in l]
+  | [G: context[if (?a <? ?b)%N then _ else _] |- _] => 
+      let l := fresh "less_than" in
+      destruct (a <? b)%N eqn:l; [apply N.ltb_lt in l| apply N.ltb_nlt in l]
+  end; inversion code1_valid; inversion code2_valid; subst; try reflexivity; try lia.
+  - specialize (N.compare_spec n1 code2) as compare_spec. 
+    destruct compare_spec; subst; try lia. 
+    apply N.lt_lt_add_r with (p:= c0800) in H. 
+    apply N.gt_lt_iff in H.
+    rewrite H. reflexivity.
+  - specialize (N.compare_spec code1 n2) as compare_spec. 
+    destruct compare_spec; subst; try lia. 
+    apply N.lt_lt_add_r with (p:= c0800) in H. 
+    rewrite H. reflexivity.
+  - specialize (N.compare_spec n1 n2) as compare_spec. 
+    destruct compare_spec; subst.
+    + rewrite N.compare_refl. reflexivity.
+    + apply N.add_lt_mono_r with (p := c0800) in H. rewrite H. reflexivity.
+    + apply N.add_lt_mono_r with (p := c0800) in H. apply N.gt_lt_iff in H. rewrite H. reflexivity.
+Qed.
+
 Definition inverse_nth_valid_codepoint (code: codepoint) : option N :=
   if (code <? cd800)%N then
     Some code
@@ -93,7 +147,8 @@ Theorem nth_valid_codepoint_invertible : forall code n,
 Proof.
   intros code n.
   split; intros.
-  - apply nth_valid_codepoint_is_some_implies_valid in H as code_valid. split; [|apply code_valid].
+  - assert (exists m, nth_valid_codepoint m = Some code). exists n. apply H.
+    apply nth_valid_codepoint_is_some_implies_valid in H0 as code_valid. split; [|apply code_valid].
     unfold inverse_nth_valid_codepoint. unfold nth_valid_codepoint in H.
     destruct (n <? cd800)%N eqn:less_than_d800.
     + inversion H. subst. rewrite less_than_d800. reflexivity.
@@ -142,21 +197,120 @@ Proof.
         -- apply N.leb_nle in plus_less_than_10ffff_m_800.
            lia.
 Qed.
-        
-Definition nth_valid_codepoint_representation (n: N) : option (list byte).
-  destruct (Nat.leb n 127) eqn:E.
-  assert (n < 255) as valid_byte. 
-  apply PeanoNat.Nat.leb_le in E. lia.
-  destruct (of_nat n) eqn:b.
-  2: { apply of_nat_None_iff in b. lia. } 
-  apply (Some [b0]).
-  apply None.
-Defined.
 
-From Coq Require Extraction.
-Extraction nth_valid_byte.
-      
-  
+Definition c07ff := N.of_hex_uint     (D7 (Df (Df Nil))).
+Definition cd800 := N.of_hex_uint (Dd (D8 (D0 (D0 Nil)))).
+Definition cffff := N.of_hex_uint (Df (Df (Df (Df Nil)))).
+
+Open Scope N_scope.
+Definition nth_valid_codepoint_representation (n: N) : option (list byte) :=
+  let n := if N.leb cd800 n then n + c0800 else n in
+  let b := fun (idx: N) => N.testbit n idx in
+  if (N.leb n 127) then
+    Some [ Byte.of_bits (b 0, (b 1, (b 2, (b 3, (b 4, (b 5, (b 6, false))))))) ]
+  else if (N.leb n c07ff) then
+    Some [ Byte.of_bits (b 6, (b 7, (b 8, (b 9, (b 10, (false, (true, true)))))));
+           Byte.of_bits (b 0, (b 1, (b 2, (b 3, (b 4,  (b 5, (false, true)))))))]
+  else if (N.leb n cffff) then
+    Some [ Byte.of_bits (b 12, (b 13, (b 14, (b 15, (false, (true, (true, true)))))));
+           Byte.of_bits (b 6,  (b 7,  (b 8,  (b 9,  (b 10, (b 11, (false, true)))))));
+           Byte.of_bits (b 0,  (b 1,  (b 2,  (b 3,  (b 4,  (b 5, (false, true)))))))]
+  else if (N.leb n c10ffff) then
+    Some [ Byte.of_bits (b 18, (b 19, (b 20, (false, (true, (true, (true, true)))))));
+           Byte.of_bits (b 12, (b 13, (b 14, (b 15, (b 16, (b 17, (false, true)))))));
+           Byte.of_bits (b 6,  (b 7,  (b 8,  (b 9,  (b 10, (b 11, (false, true)))))));
+           Byte.of_bits (b 0,  (b 1,  (b 2,  (b 3,  (b 4,  (b 5, (false, true)))))))]
+  else 
+    None.
+
+Opaque of_bits.
+
+
+
+Lemma byte_range_of_bits_00_7f: forall b1 b2 b3 b4 b5 b6 b7,
+    byte_range (Byte.of_bits (b1, (b2, (b3, (b4, (b5, (b6, (b7, false)))))))) = Range_00_7F.
+Proof.
+  intros.
+  let byte := constr:(of_bits (b1, (b2, (b3, (b4, (b5, (b6, (b7, false)))))))) in
+  pose (byte_eq := eq_refl byte);
+  apply (f_equal Byte.to_bits) in byte_eq;
+  rewrite Byte.to_bits_of_bits in byte_eq at 1;
+  destruct byte eqn:H2;
+    inversion byte_eq;
+    try reflexivity; destruct H as [G | [G | [G | G]]]; subst;
+    match goal with
+    | [F: true = false |- _] => apply Bool.diff_true_false in F; destruct F
+    end.
+Qed.
+
+Lemma byte_range_of_bits_c2_df: forall b1 b2 b3 b4 b5,
+    (b2 = true \/ b3 = true \/ b4 = true \/ b5 = true) ->
+    byte_range (Byte.of_bits (b1, (b2, (b3, (b4, (b5, (false, (true, true)))))))) = Range_C2_DF.
+Proof.
+  intros.
+  let byte := constr:(Byte.of_bits (b1, (b2, (b3, (b4, (b5, (false, (true, true)))))))) in
+  pose (byte_eq := eq_refl byte);
+  apply (f_equal Byte.to_bits) in byte_eq;
+  rewrite Byte.to_bits_of_bits in byte_eq at 1;
+  destruct byte eqn:H2; inversion byte_eq;
+    try reflexivity; destruct H as [G | [G | [G | G]]]; subst;
+    match goal with
+    | [F: true = false |- _] => apply Bool.diff_true_false in F; destruct F
+    end.
+Qed.
+
+Lemma in_range_80_bf_of_bits: forall b1 b2 b3 b4 b5 b6,
+    in_range_80_bf (of_bits (b1, (b2, (b3, (b4, (b5, (b6, (false, true)))))))).
+Proof.
+  intros.
+  let byte := constr:(Byte.of_bits (b1, (b2, (b3, (b4, (b5, (b6, (false, true)))))))) in
+  pose (byte_eq := eq_refl byte);
+  apply (f_equal Byte.to_bits) in byte_eq;
+  rewrite Byte.to_bits_of_bits in byte_eq at 1;
+  destruct byte eqn:H2; inversion byte_eq;
+    try reflexivity; destruct H as [G | [G | [G | G]]]; subst;
+    match goal with
+    | [F: true = false |- _] => apply Bool.diff_true_false in F; destruct F
+    end.
+Qed.
+
+Lemma at_least_one_bit_1 : forall n, 
+    127 < n ->
+    n <= 2047 ->
+    N.testbit n 7 = true \/ N.testbit n 8 = true \/ N.testbit n 9 = true \/ N.testbit n 10 = true.
+Proof.
+  intros.
+  Search 
+  Admitted.
+
+Lemma at_least_one_bit_2 : forall n, 
+    127 < n ->
+    n <= 2047 ->
+    N.testbit n 7 = true \/ N.testbit n 8 = true \/ N.testbit n 9 = true \/ N.testbit n 10 = true.
+Proof.
+Admitted.
+
+Theorem nth_valid_codepoint_representation_spec: forall bytes,
+    (exists n, nth_valid_codepoint_representation n = Some bytes) <->
+      valid_codepoint_representation bytes.
+Proof.
+  intros bytes. split.
+  - intros [n valid_code]. unfold nth_valid_codepoint_representation in valid_code.
+    destruct (cd800 <=? n)%N eqn:n_more_cdb00.
+    destruct (n <=? 127)%N eqn:n_less_127; [apply N.leb_le in n_less_127 | apply N.leb_nle in n_less_127].
+    + inversion valid_code. apply OneByte. apply byte_range_of_bits_00_7f.
+    + destruct (n <=? c07ff)%N eqn:n_less_07ff; [apply N.leb_le in n_less_07ff | apply N.leb_nle in n_less_07ff].
+      * inversion valid_code.
+        apply TwoByte. 2: apply in_range_80_bf_of_bits.
+        apply byte_range_of_bits_c2_df.
+        apply N.nle_gt in n_less_127.
+        clear valid_code. clear H0.
+        apply at_least_one_bit_1. apply n_less_127. apply n_less_07ff.
+      * destruct (n <=? cffff)%N eqn:n_less_ffff; [apply N.leb_le in n_less_ffff | apply N.leb_nle in n_less_ffff].
+        -- inversion valid_code. clear H0. clear valid_code. clear n_less_127.
+        
+Admitted.
+        
 
 Lemma byte_compare_antisymmetric : forall byte1 byte2, byte_compare byte1 byte2 = CompOpp (byte_compare byte2 byte1).
 Proof.
